\begin{mathpar}
\begin{array}{c}
\text{\textsc{Implication}}\\[1em]
(A \limp (B \limp A))\\
(A \limp ((A \limp B) \limp B))\\
((B \limp C) \limp ((A \limp B) \limp (A \limp C)))\\

\end{array}
\and
\begin{array}{c}
\text{\textsc{Conjunction}}\\[1em]
(A \limp (B \limp (A \land B)))\\
(A \limp (B \limp (C \limp (A \land (B \land C)))))\\
((A \land B) \limp (C \limp A))\\
((A \land B) \limp (C \limp B))\\
((A \land B) \limp (B \land A))\\

\end{array}
\and
\begin{array}{c}
\text{\textsc{Disjunction}}\\[1em]
(A \limp (A \lor B))\\
(B \limp (A \lor B))\\
(B \limp (A \lor (B \lor C)))\\
((A \lor B) \limp ((A \limp B) \limp B))\\
((A \lor B) \limp (B \lor A))\\

\end{array}
\and
\begin{array}{c}
\text{\textsc{Negation}}\\[1em]
(\bot \limp \neg A)\\
(\neg A \limp (A \limp \bot))\\
(A \limp \neg \neg A)\\
(\bot \limp A)\\
(\neg A \limp (A \limp B))\\
(A \limp ((C \limp \neg B) \limp ((A \limp B) \limp \neg C)))\\
(((A \limp B) \land (A \limp \neg B)) \limp \neg A)\\
(((A \lor \neg B) \land B) \limp A)\\
((\neg A \lor B) \limp (A \limp B))\\
((A \limp B) \limp (\neg B \limp \neg A))\\

\end{array}
\and
\begin{array}{c}
\text{\textsc{Constructive logic}}\\[1em]
((A \land B) \limp (C \limp A))\\
((A \land B) \limp (C \limp (B \land C)))\\
(A \limp (A \land (A \lor B)))\\
((A \lor (B \land C)) \limp (A \lor B))\\
((A \lor B) \limp ((A \limp B) \limp B))\\
((A \limp (B \limp C)) \limp ((A \limp B) \limp (A \limp C)))\\
((A \limp (B \limp C)) \limp ((A \land B) \limp C))\\
((A \limp B) \limp ((A \limp C) \limp (A \limp (B \land C))))\\
((A \limp B) \limp ((A \lor C) \limp (B \lor C)))\\
(((A \land B) \lor (A \lor B)) \limp (A \lor B))\\
(((A \limp C) \land (B \limp C)) \limp ((A \lor B) \limp C))\\
((\neg A \lor B) \limp (A \limp B))\\
((A \limp (B \limp C)) \limp ((A \land B) \limp C))\\
(A \limp ((A \limp B) \limp (((A \limp B) \limp (B \limp C)) \limp C)))\\
(((A \land B) \limp C) \Leftrightarrow (A \limp (B \limp C)))\\
(((A \lor B) \limp C) \Leftrightarrow ((A \limp C) \land (B \limp C)))\\

\end{array}
\and
\begin{array}{c}
\text{\textsc{Associativity}}\\[1em]
((A \land (B \land C)) \Leftrightarrow ((A \land B) \land C))\\
((A \lor (B \lor C)) \Leftrightarrow ((A \lor B) \lor C))\\

\end{array}
\and
\begin{array}{c}
\text{\textsc{Distributivity}}\\[1em]
((A \land (B \limp C)) \limp ((A \land B) \limp (A \land C)))\\
((A \land (B \lor C)) \Leftrightarrow ((A \land B) \lor (A \land C)))\\
((A \lor (B \land C)) \Leftrightarrow ((A \lor B) \land (A \lor C)))\\
(((A \limp B) \land (A \limp C)) \limp (A \limp (B \land C)))\\
((A \limp (B \land C)) \limp ((A \limp B) \land (A \limp C)))\\
(((A \limp B) \lor (A \limp C)) \limp (A \limp (B \lor C)))\\
((A \limp (B \limp C)) \limp ((A \limp B) \limp (A \limp C)))\\
(((A \limp B) \limp (A \limp C)) \limp (A \limp (B \limp C)))\\
(((A \lor B) \limp C) \Leftrightarrow ((A \limp C) \land (B \limp C)))\\

\end{array}
\and
\begin{array}{c}
\text{\textsc{\kl{Classical} logic}}\\[1em]
(((A \land B) \limp (A \land C)) \limp (A \land (B \limp C)))\\
((A \limp (B \lor C)) \limp ((A \limp B) \lor (A \limp C)))\\
(A \lor \neg A)\\
(A \lor (A \limp B))\\
((A \limp B) \lor (B \limp A))\\
(\neg \neg A \limp A)\\
(((A \limp B) \limp A) \limp A)\\
\neg \neg (A \lor \neg A)\\
\neg \neg (A \lor (A \limp B))\\
\neg \neg ((A \limp B) \lor (B \limp A))\\
\neg \neg (\neg \neg A \limp A)\\
\neg \neg (((A \limp B) \limp A) \limp A)\\

\end{array}
\and

\end{mathpar}
